WIP proof Jmp FTLR

theories/ftlr/Jmp.v
@@ -15,14 +15,251 @@ Section fundamental.
   Implicit Types w : (leibnizO Word).
   Implicit Types interp : (D).
 
-  Lemma jmp_case (r : leibnizO Reg) (p : Perm)
+
+  (*--------------------- Attempts ---------------------*)
+
+  Definition reg_allow_IE (regs : Reg) (r : RegName) (p : Perm) (b e a : Addr) :=
+    regs !! r = Some (WCap p b e a) ∧
+    p = IE /\
+    withinBounds b e a = true ∧
+    withinBounds b e (a ^+1)%a = true.
+
+  (* Mask after the jump, depending on the address of the pc and the address
+   of a *)
+  Definition mask_jmp (pc_a a : Addr) : coPset
+    :=
+    if decide (pc_a = a)
+    then (⊤ ∖ ↑logN.@pc_a ∖ ↑logN.@(a^+1)%a)
+    else
+      if decide (pc_a = (a^+1)%a)
+      then (⊤ ∖ ↑logN.@pc_a ∖ ↑logN.@a)
+      else (⊤ ∖ ↑logN.@pc_a ∖ ↑logN.@a ∖ ↑logN.@(a^+1)%a).
+
+  Definition mask_jmp_reg (regs : Reg) (r : RegName) (pc_a : Addr) (p : Perm) (b e a : Addr)
+    : coPset :=
+    if decide (reg_allow_IE regs r p b e a)
+    then mask_jmp pc_a a
+    else (⊤ ∖ ↑logN.@pc_a).
+
+  (* The necessary resources to close the region again,
+     except for the points to predicate, which we will store separately *)
+  Definition region_open_resources2
+    (pc_a : Addr) (a : Addr)
+    (w1 : Word) (w2 : Word)
+    (P1 P2 : D)
+    : iProp Σ :=
+    (▷ P1 w1 ∗ ▷ P2 w2
+       ∗ ((▷ ∃ w1 w2, a ↦ₐ w1 ∗ P1 w1 ∗ (a^+1)%a ↦ₐ w2 ∗ P2 w2)
+          ={mask_jmp pc_a a, ⊤ ∖ ↑logN.@pc_a}=∗ emp))%I.
+
+  Definition region_open_resources
+    (pc_a : Addr) (a : Addr) (w : Word)
+    (P : D)
+    : iProp Σ :=
+    (▷ P w ∗
+       ((▷ ∃ w, a ↦ₐ w ∗ P w)
+        ={mask_jmp pc_a a, ⊤ ∖ ↑logN.@pc_a}=∗ emp))%I.
+
+  Definition region_open_resources'
+    (pc_a : Addr) (a : Addr) (w' : Word)
+    (P : D)
+    : iProp Σ :=
+    (▷ P w' ∗
+       ((▷ ∃ w', (a^+1)%a ↦ₐ w' ∗ P w')
+        ={mask_jmp pc_a a, ⊤ ∖ ↑logN.@pc_a}=∗ emp))%I.
+
+  (* Description of what the resources are supposed to look like after opening the
+     region if we need to, but before closing the region up again*)
+  Definition allow_IE_res (regs : Reg) (r : RegName)
+    (pc_a : Addr) (p : Perm) (b e a : Addr)
+    (P1 P2 : D) : iProp Σ :=
+    (⌜read_reg_inr regs r p b e a⌝ ∗
+
+       if decide (reg_allow_IE regs r p b e a)
+       then
+         |={⊤ ∖ ↑logN.@pc_a, mask_jmp pc_a a}=>
+           (if decide (pc_a = a)
+            then ∃ w2, (a^+1)%a ↦ₐ w2 ∗ region_open_resources' pc_a a w2 P2
+            else
+              if decide (pc_a = (a^+1)%a)
+              then ∃ w1, a ↦ₐ w1 ∗ region_open_resources pc_a a w1 P1
+              else ∃ w1 w2, a ↦ₐ w1 ∗ (a^+1)%a ↦ₐ w2 ∗ region_open_resources2 pc_a a w1 w2 P1 P2
+           )
+       else True)%I.
+
+  Definition allow_IE_mem
+    (regs : Reg) (r : RegName)
+    (pc_a : Addr) (pc_w : Word) (mem : Mem) (p : Perm) (b e a : Addr) (P1 P2 : D) :=
+    (⌜read_reg_inr regs r IE b e a⌝ ∗
+       if decide (reg_allow_IE regs r p b e a)
+       then (if decide (pc_a = a)
+             then ∃ w2, ⌜mem = <[(a^+1)%a:=w2]> (<[pc_a:=pc_w]> ∅)⌝ ∗ region_open_resources' pc_a a w2 P2
+             else
+               if decide (pc_a = (a^+1)%a)
+               then ∃ w1, ⌜mem = <[a:=w1]> (<[pc_a:=pc_w]> ∅)⌝ ∗ region_open_resources pc_a a w1 P1
+               else ∃ w1 w2,
+                   ⌜mem = <[(a^+1)%a:=w2]> (<[a:=w1]> (<[pc_a:=pc_w]> ∅))⌝
+                                             ∗ region_open_resources2 pc_a a w1 w2 P1 P2)
+       else ⌜mem = <[pc_a:=pc_w]> ∅⌝)%I.
+
+  Lemma create_IE_res:
+    ∀ (regs : leibnizO Reg) (r : RegName)
+      (pc_p : Perm) (pc_b pc_e pc_a : Addr)
+      (widc : Word)
+      (p : Perm) (b e a : Addr),
+      read_reg_inr (<[PC:=WCap pc_p pc_b pc_e pc_a]> (<[idc:= widc]> regs)) r p b e a
+      → (∀ (r' : RegName) (w : Word), ⌜r' ≠ PC⌝ → ⌜r' ≠ idc⌝ → ⌜regs !! r' = Some w⌝ → (fixpoint interp1) w)
+        -∗ interp widc
+        -∗ ∃ (P1 P2 : D),
+             allow_IE_res (<[PC:=WCap pc_p pc_b pc_e pc_a]> (<[idc:=widc]> regs)) r pc_a p b e a P1 P2.
+  Proof.
+    intros regs r pc_p pc_b pc_e pc_a widc p b e a HVr.
+    iIntros "#Hreg #Hwidc".
+    iFrame "%".
+    case_decide as Hallows; cycle 1.
+    - by iExists (λne _, True%I), (λne _, True%I).
+    - rewrite /mask_jmp.
+      destruct Hallows as (Hreg & -> & Hwb & Hwb').
+      assert (a <> (a^+1)%a) by (apply andb_prop in Hwb as [_ Hge]; solve_addr).
+      apply Is_true_true_2 in Hwb, Hwb'.
+      assert ( withinBounds b e a /\ withinBounds b e (a^+1)%a) as Hwbs by auto.
+      case_decide as Ha; simplify_eq.
+      {
+      admit.
+      }
+      apply neq_Symmetric in Ha.
+      assert (r ≠ PC) as Hneq.
+      { refine (addr_ne_reg_ne Hreg _ Ha). by simplify_map_eq. }
+
+      case_decide as Ha'; simplify_eq.
+      {
+      admit.
+      }
+
+      (* apply andb_prop in Hwb as [Hle Hge]. *)
+      (* revert Hle Hge. rewrite !Z.leb_le Z.ltb_lt =>Hle Hge. *)
+      (* apply andb_prop in Hwb' as [Hle' Hge']. *)
+      (* revert Hle' Hge'. rewrite !Z.leb_le Z.ltb_lt =>Hle' Hge'. *)
+
+
+      rewrite lookup_insert_ne //= in Hreg.
+      destruct (decide (r = idc)) as [|Hneq']; simplify_map_eq.
+      + rewrite fixpoint_interp1_eq /=.
+        iDestruct ("Hwidc" $! Hwbs) as (P1 P2) "(Hpers_P1 & Hpers_P2 & Hinv_a & Hinv_a' & _)".
+        iExists P1, P2.
+
+        iMod (inv_acc (⊤ ∖ ↑logN.@pc_a) with "Hinv_a") as "[Hrefinv_a Hcls_a]";[solve_ndisj|].
+        iMod (inv_acc (⊤ ∖ ↑logN.@pc_a ∖ ↑logN.@a) with "Hinv_a'") as "[Hrefinv_a' Hcls_a']";[solve_ndisj|].
+        iDestruct "Hrefinv_a" as (w1) "[>Ha HPa]".
+        iDestruct "Hrefinv_a'" as (w2) "[>Ha' HPa']".
+        iExists w1, w2.
+
+        iFrame "∗ #".
+        rewrite /region_open_resources2.
+        iModIntro.
+        iIntros "Ha".
+        iDestruct "Ha" as (w1' w2') "(Hw1' & HP1' & Hw2' & HP2')".
+        rewrite /mask_jmp.
+        case_decide; simplify_eq.
+        case_decide; simplify_eq.
+        iMod ("Hcls_a'" with "[Hw2' HP2']") as "_"; first (iExists _ ; iFrame).
+        iMod ("Hcls_a" with "[Hw1' HP1']") as "_"; first (iExists _ ; iFrame).
+        done.
+      + iDestruct ("Hreg" $! r _ Hneq Hneq' Hreg) as "Hvsrc".
+        rewrite (fixpoint_interp1_eq (WCap _ _ _ _)) /=.
+        iDestruct ("Hvsrc" $! Hwbs) as (P1 P2) "(Hpers_P1 & Hpers_P2 & Hinv_a & Hinv_a' & _)".
+        iExists P1, P2.
+
+        iMod (inv_acc (⊤ ∖ ↑logN.@pc_a) with "Hinv_a") as "[Hrefinv_a Hcls_a]";[solve_ndisj|].
+        iMod (inv_acc (⊤ ∖ ↑logN.@pc_a ∖ ↑logN.@a) with "Hinv_a'") as "[Hrefinv_a' Hcls_a']";[solve_ndisj|].
+        iDestruct "Hrefinv_a" as (w1) "[>Ha HPa]".
+        iDestruct "Hrefinv_a'" as (w2) "[>Ha' HPa']".
+        iExists w1, w2.
+
+        iFrame "∗ #".
+        rewrite /region_open_resources2.
+        iModIntro.
+        iIntros "Ha".
+        iDestruct "Ha" as (w1' w2') "(Hw1' & HP1' & Hw2' & HP2')".
+        rewrite /mask_jmp.
+        case_decide; simplify_eq.
+        case_decide; simplify_eq.
+        iMod ("Hcls_a'" with "[Hw2' HP2']") as "_"; first (iExists _ ; iFrame).
+        iMod ("Hcls_a" with "[Hw1' HP1']") as "_"; first (iExists _ ; iFrame).
+        done.
+  Admitted.
+
+  (*--------------------- Defs from rules_jmp.v ---------------------*)
+  (* Definition allow_load_addr_or_true (b e a : Addr) (mem : Mem):= *)
+  (*   if decide (withinBounds b e a = true) *)
+  (*   then ∃ w, mem !! a = Some w *)
+  (*   else True. *)
+
+  (* Definition allow_IE_map_or_true (r : RegName) (regs : Reg) (mem : Mem) := *)
+  (*   ∃ p b e a, *)
+  (*     read_reg_inr regs r p b e a ∧ (* unify the content of `r` with cap (p,b,e,a) *) *)
+  (*       allow_load_addr_or_true b e a mem /\ (* b ≤ a < e, and mem(a) = w *) *)
+  (*       allow_load_addr_or_true b e (a^+1)%a mem. *)
+
+  (* Definition allow_IE_cap (r : RegName) (regs : Reg) (mem : Mem) := *)
+  (*   forall wr, regs !! r = Some wr -> *)
+  (*         is_ie_cap wr -> *)
+  (*         is_Some (regs !! idc) /\ allow_IE_map_or_true r regs mem. *)
+
+
+  (*--------------------- Defs from rules_jmp.v ---------------------*)
+
+  (* Definition reg_allows_store (regs : Reg) (r : RegName) p b e a := *)
+  (*   regs !! r = Some (WCap p b e a) ∧ *)
+  (*   writeAllowed p = true ∧ withinBounds b e a = true. *)
+
+        (* if decide (reg_allows_store r r1 p1 b1 e1 a0 ∧ a0 ≠ a) *)
+        (* then ⊤ ∖ ↑logN.@a ∖ ↑logN.@a0 *)
+        (* else ⊤ ∖ ↑logN.@a}=∗ *)
+        (*                      ∃ mem0 : gmap Addr Word, *)
+
+
+  (*--------------------- Lemma ---------------------*)
+
+  Lemma jmp_case (regs : leibnizO Reg) (p : Perm)
         (b e a : Addr) (widc w : Word) (src : RegName) (P : D):
-    ftlr_instr r p b e a widc w (Jmp src) P.
+    ftlr_instr regs p b e a widc w (Jmp src) P.
   Proof.
     intros Hp Hsome i Hbae Hi.
     iIntros
       "#IH #Hinv_pc #Hinv_idc #Hinva #Hreg #Hread Hown Ha HP Hcls HPC HIDC Hmap".
-    iInsert "Hmap" idc.
+    iInsertList "Hmap" [idc;PC].
+
+    (* To read out PC's name later, and needed when calling wp_load *)
+    assert(∀ x : RegName, is_Some (<[PC:=WCap p b e a]> (<[idc:=widc]> regs) !! x)) as Hsome'.
+    {
+      intros. destruct (decide (x = PC)).
+      rewrite e0 lookup_insert; unfold is_Some. by eexists.
+      destruct (decide (x = idc)).
+      rewrite lookup_insert_ne; auto.
+      rewrite e0 lookup_insert; unfold is_Some. by eexists.
+      by rewrite! lookup_insert_ne.
+    }
+
+    (* Initializing the names for the values of Hsrc now, to instantiate the existentials in step 1 *)
+    assert (∃ p0 b0 e0 a0, read_reg_inr (<[PC:=WCap p b e a]> (<[idc:=widc]> regs)) src p0 b0 e0 a0)
+      as [p0 [b0 [e0 [a0 HVsrc] ] ] ].
+    {
+      specialize Hsome' with src as Hsrc.
+      destruct Hsrc as [wsrc Hsomesrc].
+      unfold read_reg_inr. rewrite Hsomesrc.
+      destruct wsrc as [|[ p0 b0 e0 a0|] | ]; try done.
+      by repeat eexists.
+    }
+
+    (* Step 1: open the region, if necessary, and store all the resources
+       obtained from the region in allow_IE_res *)
+    iDestruct (create_IE_res with "Hreg Hinv_idc") as (P1 P2) "HJmpRes"; eauto.
+
+    (* WIP.... *)
+
+    Admitted.
+
 
     destruct (decide (src = PC)); simplify_map_eq.
     - iApply (wp_jmp_successPC with "[HPC Ha]"); eauto; first iFrame.
@@ -40,7 +277,12 @@ Section fundamental.
 
     - destruct (decide (src = idc)); simplify_map_eq.
       + admit. (* TODO need the wp_rule.... *)
-      + specialize Hsome with src as Hsrc.
+      + iInsertList "Hmap" [PC].
+        iAssert ([∗ map] k↦x ∈ (<[a := w]> ∅), k ↦ₐ x)%I with "[Ha]" as "Hmem".
+        { iApply (big_sepM_insert with "[Ha]"); auto ; iFrame. }
+
+
+        specialize Hsome with src as Hsrc.
         destruct Hsrc as [wsrc Hsomesrc].
         iExtractList "Hmap" [src;idc] as ["Hsrc";"Hidc"].
         iAssert (fixpoint interp1 wsrc) as "#Hinv_src"; first (iApply "Hreg"; eauto).
@@ -58,6 +300,8 @@ Section fundamental.
             (* TODO we can probably encode the disjunction in a better way *)
             destruct Hdec_wb as [ Hwb%Is_true_true_1 Hwb'%Is_true_true_1].
             assert (a' ≠ (a' ^+1)%a) by (rewrite withinBounds_true_iff in Hwb'; solve_addr).
+
+
             destruct (decide (a = a')) as [Haeq|Haeq];
               destruct (decide (a = (a' ^+1)%a)) as [Haeq'|Haeq'].
             ** (* a' = a , a = a ^+ 1*) solve_addr.
